Wavelet.lean
@@ -2,3 +2,6 @@ import Wavelet.Semantics
 import Wavelet.Seq
 import Wavelet.Dataflow
 import Wavelet.Compile
+
+-- TODO: move this to better places
+import Wavelet.Determinacy
